Work on Veriloggen proof

src/translation/Veriloggenproof.v
@@ -16,16 +16,64 @@
  * along with this program.  If not, see <https://www.gnu.org/licenses/>.
  *)
 
-From compcert Require Import Smallstep.
+From compcert Require Import Smallstep Linking.
+From coqup Require Import Veriloggen.
 From coqup Require HTL Verilog.
+
+Definition match_prog (prog : HTL.program) (tprog : Verilog.program) :=
+  match_program (fun cu f tf => tf = transl_fundef f) eq prog tprog.
+
+Lemma transf_program_match:
+  forall prog, match_prog prog (transl_program prog).
+Proof.
+  intros. eapply match_transform_program_contextual. auto.
+Qed.
+
+Inductive match_stacks : list HTL.stackframe -> list Verilog.stackframe -> Prop :=
+| match_stack :
+    forall res m pc reg_assoc arr_assoc hstk vstk,
+      match_stacks hstk vstk ->
+      match_stacks (HTL.Stackframe res m pc reg_assoc arr_assoc :: hstk)
+                   (Verilog.Stackframe res (transl_module m) pc
+                                       reg_assoc arr_assoc :: vstk)
+| match_stack_nil : match_stacks nil nil.
+
+Inductive match_states : HTL.state -> Verilog.state -> Prop :=
+| match_state :
+    forall m st reg_assoc arr_assoc hstk vstk,
+      match_stacks hstk vstk ->
+      match_states (HTL.State hstk m st reg_assoc arr_assoc)
+                   (Verilog.State vstk (transl_module m) st reg_assoc arr_assoc)
+| match_returnstate :
+    forall v hstk vstk,
+      match_stacks hstk vstk ->
+      match_states (HTL.Returnstate hstk v) (Verilog.Returnstate vstk v)
+| match_initial_call :
+    forall m,
+      match_states (HTL.Callstate nil m nil) (Verilog.Callstate nil (transl_module m) nil).
 
 Section CORRECTNESS.
 
   Variable prog: HTL.program.
   Variable tprog: Verilog.program.
 
+  Hypothesis TRANSL : match_prog prog tprog.
+
+  Let ge : HTL.genv := Globalenvs.Genv.globalenv prog.
+  Let tge : Verilog.genv := Globalenvs.Genv.globalenv tprog.
+
+  Theorem transl_step_correct:
+    forall (S1 : HTL.state) t S2,
+      HTL.step ge S1 t S2 ->
+      forall (R1 : Verilog.state),
+        match_states S1 R1 ->
+        exists R2, Smallstep.plus Verilog.step tge R1 t R2 /\ match_states S2 R2.
+  Proof.
+    induction 1; intros R1 MSTATE.
+
   Theorem transf_program_correct:
     forward_simulation (HTL.semantics prog) (Verilog.semantics tprog).
-  Admitted.
+
 
 End CORRECTNESS.
+
